\documentclass[11pt, oneside]{article}   	% use "amsart" instead of "article" for AMSLaTeX format
\usepackage{geometry}                		% See geometry.pdf to learn the layout options. There are lots.
\geometry{letterpaper}                   		% ... or a4paper or a5paper or ... 
%\geometry{landscape}                		% Activate for for rotated page geometry
%\usepackage[parfill]{parskip}    		% Activate to begin paragraphs with an empty line rather than an indent
\usepackage{graphicx}				% Use pdf, png, jpg, or epsÂ§ with pdflatex; use eps in DVI mode
								% TeX will automatically convert eps --> pdf in pdflatex		
\usepackage{amssymb}

\title{Driven linear collisionless gyrokinetics with  $\delta B_\parallel = 0$}
\author{Yuguang Tong}
%\date{}							% Activate to display a given date or no date
\begin{document}
\newcommand{\vect}[1]{\mathbf{#1}}

\maketitle
\section{Set up}
We start fro the Laplace-Fourier solution given in the AstroGK manual, i.e., Eq. (6.124):
%
\begin{equation}
\hat{A}_{\parallel \vect{k}}(p) = \frac{-Q^2 A_{\parallel \vect{k}_0}}{\left(p^2 + Q^2 \right) (p + i\omega_0)}
\end{equation}
where
%
\begin{equation}
Q^2(p) = \frac{\alpha_i A k_\parallel^2 v_A^2}{AB-B^2}
\end{equation}
and 
%
\begin{eqnarray}
A &=& \sum_s \frac{T_i}{T_s} (1 + \Gamma_{0s} \xi_s Z_s) \\
B &=& \sum_s \frac{T_i}{T_s} ( 1 - \Gamma_{0s})
\end{eqnarray}
$\alpha_s = k_\perp^2 \rho_s^2 / 2$ and $\xi_s = ip/kv_{ts}$

$p^2 + Q^2$ is just the dispersion relation. The system with $\delta B_\parallel = 0$ has two solutions, both Alfv{\'e}n waves. We denote the two solutions $p_1 = -i\omega_1$ and $p_2 = p_1^* = -i \omega_2 = i \omega_1^*$. AstroGK manual approximates $p^2 + Q^2$ by $(p-p_1)(p-p_2)$. 

\section{Inverse Laplace transform}
We take a different path here and directly evaluate the inverse Laplace transform via Bromwich integral. 

%
\begin{eqnarray}
A_{\parallel\vect{k}} &=& \mathrm{ILT}\left(\hat{A}_{\parallel \vect{k}}\right (p)) \\
&=& \frac{1}{2\pi i} \int_{\beta-i\infty}^{\beta + i \infty} \frac{-Q^2 e^{pt}}{(p^2+Q^2)(p+i\omega_0)} dp \\
&=& \mathrm{Res}(p_1) + \mathrm{Res}(p_2) + \mathrm{Res}(p = - i\omega_0) 
\end{eqnarray}
where $\mathrm{Res}$ denotes residue.

The residue at $p_0 = - i\omega_0$ is trivially 
%
\begin{equation}
\mathrm{Res}(p = - i\omega_0)  = \left[\frac{-Q^2}{p^2 + Q^2} \right]_{p=-i\omega_0}
\end{equation}
The residues at $p_1$ and $p_2$ are evaluated by
%
\begin{eqnarray}
\mathrm{Res}(p_1)&=& \left[ (p-p_1) \frac{-Q^2 e^{pt}}{(p^2+Q^2)(p+i\omega_0)} \right]_{p=p_1} \\
&=& \frac{-Q^2(p_1) e^{p_1t}}{\left[\frac{d (p^2+Q^2)}{dp} +  \sum_{n=2}^\infty \frac{1}{n!} \frac{d^n(p^2+Q^2)}{dp^n} (p-p_1)^n \right]_{p=p_1}(p_1 + i\omega_0)} \\
&=& \frac{-Q^2(p_1) e^{p_1t}}{\left[\frac{d (p^2+Q^2)}{dp} \right]_{p=p_1}(p_1 + i\omega_0)} \\
\end{eqnarray}
and
%
\begin{equation}
p_1 \leftrightarrow p_2
\end{equation}

For convenience to compare with simulation, we introduce the dimensionless frequency 
%
\begin{eqnarray}
\overline{\omega} &=& \frac{\omega}{k_\parallel v_A} = \frac{p}{-i k_\parallel v_A} \\
\overline{t} &=& k_\parallel v_A t
\end{eqnarray}
Therefore 
%
\begin{equation}
\xi_s = \sqrt{\frac{T_i}{T_s}\frac{m_s}{m_i}} \frac{\overline{\omega}}{\sqrt{\beta_I}}
\end{equation}

The dimensionless dispersion relation takes the form:
\begin{equation}
\overline{\omega}^2 - \overline{Q}^2= 0
\end{equation}
where 
\begin{equation}
\overline{Q}^2 = \frac{Q^2}{-k_\parallel^2 v_A^2} =  \frac{\alpha_i A}{(A-B)B} 
\end{equation}

Hence the residue $\mathrm{Res}(p=-i\omega_0)$ becomes
%
\begin{equation}
\mathrm{Res}(\overline{\omega}_0) = \frac{\overline{Q}^2(\overline{\omega}_0) e^{-i \overline{\omega}_0 \overline{t}}}{\overline{\omega}_0 ^2 - \overline{Q}^2(\overline{\omega}_0)}
\end{equation}

The residues of the other two poles are 
\begin{equation}
\mathrm{Res}(\overline{\omega}_j) = \frac{\overline{Q}^2(\overline{\omega}_j) e^{-i \overline{\omega}_j \overline{t}}}{(G(\overline{\omega}_j) + 2 \overline{\omega}_j)(\overline{\omega}_j  - \overline{\omega}_0)}
\end{equation}
where $j = 1, 2$ and 
\begin{equation}
G =  \frac{\alpha_i}{\sqrt{\beta_i} (A-B)^2} \sum_s \left(\frac{T_i}{T_s}\right)^{3/2} \sqrt{\frac{m_s}{m_i}} \Gamma_{0s} \left[(1-2\xi_s^2)Z_s - 2 \xi_s\right]
\end{equation}

\end{document}  